rust/opendp_verified/OpenDPVerified.lean
@@ -1,3 +1,4 @@
 import src.samplers.uniform.mod
+import src.utilities.mod
 import src.samplers.bernoulli.mod
 import src.measurements.noisy_top_k
